inline ossl3::support and ossl3::error in ossl3 to rmeove cycle dependencies.

rust/implementation/openssl3/mod.rs
@@ -39,6 +39,7 @@ const OQS_PROVIDER_NAME_PTR: *const c_char = (OQS_PROVIDER_NAME as *const u8).ca
 /// A wrapper around an `OSSL_PROVIDER`.
 struct Provider<'a>(Pimpl<'a, openssl3::OSSL_PROVIDER>);
 
+#[hax_lib::exclude]
 impl std::fmt::Debug for Provider<'_> {
     fn fmt(&self, f: &mut std::fmt::Formatter) -> std::fmt::Result {
         write!(f, "Provider({:p}", self.0.as_nonnull().as_ptr())
@@ -110,7 +111,7 @@ impl ProviderBuilder {
         .ok_or_else(|| {
             (
                 pb::SystemError::SYSTEMERROR_BACKEND,
-                format!("failed to load provider: {}", support::errstr()),
+                format!("failed to load provider: {}", crate::ossl3::errstr()),
             )
         })?;
 
@@ -162,7 +163,7 @@ impl<'a> LibCtx<'a> {
         {
             return Err((
                 pb::SystemError::SYSTEMERROR_MEMORY,
-                format!("failed to add the oqsprovider: {}", support::errstr()),
+                format!("failed to add the oqsprovider: {}", crate::ossl3::errstr()),
             )
                 .into());
         }
@@ -214,9 +215,712 @@ impl<'a> LibCtx<'a> {
     }
 }
 
+pub(crate) use openssl3::{
+    BIO as NativeBio, EVP_PKEY as NativePrivateKey, SSL as NativeSsl, SSL_CTX as NativeSslCtx,
+    X509 as NativeX509Certificate, X509_STORE_CTX as NativeX509StoreCtx,
+    X509_VERIFY_PARAM as NativeX509VerifyParam,
+};
+
+use std::ffi::{c_int, c_ulong, CStr, CString};
+use std::ptr::{self};
+
+
+/// Returns the last error.
+pub(crate) fn peek_last_error() -> c_ulong {
+    unsafe { openssl3::ERR_peek_last_error() }
+}
+
+/// Returns the library where a given error occurred.
+///
+/// This function reproduces the `ERR_GET_LIB` method from OpenSSL, which
+/// is a static function in header (thus not understandable by bindgen).
+pub(crate) fn err_get_lib(err: c_ulong) -> c_int {
+    ((err >> openssl3::ERR_LIB_OFFSET) & (openssl3::ERR_LIB_MASK as c_ulong)) as c_int
+}
+
+/// Returns the reason of why a given error occurred.
+///
+/// This function reproduces the `ERR_GET_REASON` method from OpenSSL, which
+/// is a static function in header (thus not understandable by bindgen).
+pub(crate) fn err_get_reason(err: c_ulong) -> c_int {
+    (err & (openssl3::ERR_REASON_MASK as c_ulong)) as c_int
+}
+
+/// Returns a string containing the error strings for all errors that
+/// OpenSSL 3 has recorded.
+/// This function clears the error queue.
+pub(crate) fn errstr() -> String {
+    const DEFAULT_BUFFER_LEN: usize = 256;
+
+    let Some(bio) = (unsafe {
+        Pimpl::new(openssl3::BIO_new(openssl3::BIO_s_mem()), |x| {
+            openssl3::BIO_free_all(x)
+        })
+    }) else {
+        return "unknown error (BIO unavailable)".into();
+    };
+
+    unsafe {
+        openssl3::ERR_print_errors(bio.as_nonnull().as_ptr());
+    }
+
+    let mut buffer = vec![0u8; DEFAULT_BUFFER_LEN];
+
+    let mut buffer_ptr = buffer.as_mut_ptr();
+    let mut size = 0;
+    loop {
+        let mut readbytes = 0usize;
+        let ret = unsafe {
+            openssl3::BIO_read_ex(
+                bio.as_nonnull().as_ptr(),
+                buffer_ptr.cast(),
+                DEFAULT_BUFFER_LEN,
+                &mut readbytes as *mut _,
+            )
+        };
+        if ret == 0 {
+            break;
+        }
+        if readbytes == 0 {
+            break;
+        }
+        size += readbytes;
+        if readbytes < DEFAULT_BUFFER_LEN {
+            break;
+        }
+        let current_position = buffer.len();
+        let Some(new_size) = current_position.checked_add(DEFAULT_BUFFER_LEN) else {
+            break;
+        };
+        buffer.resize(new_size, 0u8);
+        buffer_ptr = unsafe { buffer.as_mut_ptr().add(current_position) };
+    }
+    buffer.resize(size, 0u8);
+
+    if let Some(first_null_byte) = buffer.iter().position(|x| *x == 0u8) {
+        if first_null_byte == 0 {
+            return "no additional information".to_string();
+        }
+        buffer.resize(first_null_byte, 0u8);
+    } else if buffer.is_empty() {
+        return "no additional information".to_string();
+    }
+
+    String::from_utf8(buffer).unwrap_or_else(|_| "unknown error (not UTF-8)".into())
+}
+
+/// Creates a new `BIO` object with a specific method.
+#[allow(non_snake_case)]
+pub(crate) fn new_BIO(
+    bio_meth: NonNull<openssl3::BIO_METHOD>,
+) -> crate::Result<Pimpl<'static, NativeBio>> {
+    unsafe {
+        Pimpl::new(openssl3::BIO_new(bio_meth.as_ptr()), |bio| {
+            openssl3::BIO_free_all(bio)
+        })
+    }
+    .ok_or_else(|| {
+        (
+            pb::SystemError::SYSTEMERROR_MEMORY,
+            "failed to create a new BIO object",
+        )
+            .into()
+    })
+}
+
+/// Creates a `BIO` object from a immutable buffer.
+#[allow(non_snake_case)]
+pub(crate) fn BIO_from_buffer<'a>(buffer: impl AsRef<[u8]> + 'a) -> crate::Result<Pimpl<'a, NativeBio>> {
+    let buffer = buffer.as_ref();
+    let size: i32 = buffer.len().try_into().map_err(|e| {
+        (
+            pb::SystemError::SYSTEMERROR_INTEGER_OVERFLOW,
+            format!("cannot create a BIO object: {e}"),
+        )
+    })?;
+    unsafe {
+        Pimpl::new(
+            openssl3::BIO_new_mem_buf(buffer.as_ptr().cast(), size),
+            |x| openssl3::BIO_free_all(x),
+        )
+    }
+    .ok_or_else(|| {
+        (
+            pb::SystemError::SYSTEMERROR_MEMORY,
+            "cannot allocate a new BIO object",
+        )
+            .into()
+    })
+}
+
+/// Reads a certificate (`X509` object) from a `BIO` object.
+#[allow(non_snake_case)]
+pub(crate) fn X509_from_BIO<'a, 'b>(
+    lib_ctx: &'_ LibCtx<'a>,
+    bio: NonNull<NativeBio>,
+    format: pb_api::ASN1EncodingFormat,
+) -> crate::Result<Pimpl<'b, openssl3::X509>>
+where
+    'a: 'b,
+{
+    let x509 =
+        NonNull::new(unsafe { openssl3::X509_new_ex(lib_ctx.as_nonnull().as_ptr(), ptr::null()) })
+            .ok_or((
+                pb::SystemError::SYSTEMERROR_MEMORY,
+                "failed to allocate a new `X509` object",
+            ))?;
+
+    let mut inplace_ptr = x509.as_ptr();
+    let ptr = match format {
+        pb_api::ASN1EncodingFormat::ENCODING_FORMAT_PEM => {
+            NonNull::new(unsafe {
+                openssl3::PEM_read_bio_X509(bio.as_ptr(), &mut inplace_ptr, None, ptr::null_mut())
+            })
+            .ok_or_else(|| {
+                unsafe { openssl3::X509_free(inplace_ptr) };
+                (
+                    pb::CertificateError::CERTIFICATEERROR_MALFORMED,
+                    format!("failed to read the certificate: {}", errstr()),
+                )
+            })?;
+            inplace_ptr
+        }
+        pb_api::ASN1EncodingFormat::ENCODING_FORMAT_DER => {
+            NonNull::new(unsafe { openssl3::d2i_X509_bio(bio.as_ptr(), &mut inplace_ptr) })
+                .ok_or_else(|| {
+                    unsafe { openssl3::X509_free(inplace_ptr) };
+                    (
+                        pb::CertificateError::CERTIFICATEERROR_MALFORMED,
+                        format!("failed to read the certificate: {}", errstr()),
+                    )
+                })?;
+            inplace_ptr
+        }
+    };
+    Ok(unsafe { Pimpl::new_unchecked(ptr, |x| openssl3::X509_free(x)) })
+}
+
+/// Reads a private key (`EVP_PKEY` object) from a `BIO` object.
+#[allow(non_snake_case)]
+pub(crate) fn EVP_PKEY_from_BIO<'a, 'b>(
+    lib_ctx: &'_ LibCtx<'a>,
+    bio: NonNull<NativeBio>,
+    format: pb_api::ASN1EncodingFormat,
+) -> crate::Result<Pimpl<'b, openssl3::EVP_PKEY>>
+where
+    'a: 'b,
+{
+    unsafe {
+        Pimpl::new(
+            match format {
+                pb_api::ASN1EncodingFormat::ENCODING_FORMAT_PEM => {
+                    openssl3::PEM_read_bio_PrivateKey_ex(
+                        bio.as_ptr(),
+                        ptr::null_mut(),
+                        None,
+                        ptr::null_mut(),
+                        lib_ctx.as_nonnull().as_ptr(),
+                        ptr::null(),
+                    )
+                }
+                pb_api::ASN1EncodingFormat::ENCODING_FORMAT_DER => openssl3::d2i_PrivateKey_ex_bio(
+                    bio.as_ptr(),
+                    ptr::null_mut(),
+                    lib_ctx.as_nonnull().as_ptr(),
+                    ptr::null(),
+                ),
+            },
+            |x| openssl3::EVP_PKEY_free(x),
+        )
+    }
+    .ok_or_else(|| {
+        (
+            pb::PrivateKeyError::PRIVATEKEYERROR_MALFORMED,
+            format!("failed to read the private key: {}", errstr()),
+        )
+            .into()
+    })
+}
+
+/// Tells if a BIO has reached EOF.
+#[allow(non_snake_case)]
+pub(crate) fn is_BIO_eof(bio: NonNull<NativeBio>) -> bool {
+    // `BIO_eof` is a C macro.
+    (unsafe {
+        openssl3::BIO_ctrl(
+            bio.as_ptr(),
+            openssl3::BIO_CTRL_EOF as c_int,
+            0,
+            ptr::null_mut(),
+        )
+    }) == 1
+}
+
+/// Returns the cipher name in the OpenSSL format.
+pub(crate) fn cipher_name(name: impl AsRef<str>) -> Option<&'static str> {
+    let cstr = CString::new(name.as_ref().to_string()).ok()?;
+    NonNull::new(unsafe { openssl3::OPENSSL_cipher_name(cstr.as_ptr()) }.cast_mut())
+        .and_then(|nn| unsafe { CStr::from_ptr(nn.as_ptr()) }.to_str().ok())
+}
+
+macro_rules! gen_enum_from_openssl {
+    ( $name:ident, $doc:expr, $( ($sym:ident, $value:ident)$(,)? )* ) => {
+        #[derive(Debug, PartialEq, Eq, Copy, Clone)]
+        #[doc=$doc]
+        #[allow(dead_code)]
+        #[repr(isize)]
+        pub(crate) enum $name {
+            $(
+                $sym = ::openssl3::$value as isize,
+            )*
+        }
+
+        impl TryFrom<::std::ffi::c_int> for $name {
+            type Error = ();
+
+            fn try_from(err: ::std::ffi::c_int) -> Result<Self, Self::Error> {
+                #[allow(unreachable_patterns)]
+                match err as u32 {
+                    $(
+                        openssl3::$value => Ok(Self::$sym),
+                    )*
+                        _ => Err(())
+                }
+            }
+        }
+    };
+}
+
+gen_enum_from_openssl!(
+    ErrorLibrary,
+    "Library where an error can occur",
+    (None, ERR_LIB_NONE),
+    (Sys, ERR_LIB_SYS),
+    (Bn, ERR_LIB_BN),
+    (Rsa, ERR_LIB_RSA),
+    (Dh, ERR_LIB_DH),
+    (Evp, ERR_LIB_EVP),
+    (Buf, ERR_LIB_BUF),
+    (Obj, ERR_LIB_OBJ),
+    (Pem, ERR_LIB_PEM),
+    (Dsa, ERR_LIB_DSA),
+    (X509, ERR_LIB_X509),
+    (Asn1, ERR_LIB_ASN1),
+    (Conf, ERR_LIB_CONF),
+    (Crypto, ERR_LIB_CRYPTO),
+    (Ec, ERR_LIB_EC),
+    (Ssl, ERR_LIB_SSL),
+    (Bio, ERR_LIB_BIO),
+    (Pkcs7, ERR_LIB_PKCS7),
+    (X509v3, ERR_LIB_X509V3),
+    (Pkcs12, ERR_LIB_PKCS12),
+    (Rand, ERR_LIB_RAND),
+    (Dso, ERR_LIB_DSO),
+    (Engine, ERR_LIB_ENGINE),
+    (Ocsp, ERR_LIB_OCSP),
+    (Ui, ERR_LIB_UI),
+    (Comp, ERR_LIB_COMP),
+    (Ecdsa, ERR_LIB_ECDSA),
+    (Ecdh, ERR_LIB_ECDH),
+    (OsslStore, ERR_LIB_OSSL_STORE),
+    (Fips, ERR_LIB_FIPS),
+    (Cms, ERR_LIB_CMS),
+    (Ts, ERR_LIB_TS),
+    (Hmac, ERR_LIB_HMAC),
+    (Ct, ERR_LIB_CT),
+    (Async, ERR_LIB_ASYNC),
+    (Kdf, ERR_LIB_KDF),
+    (Sm2, ERR_LIB_SM2),
+    (Ess, ERR_LIB_ESS),
+    (Prop, ERR_LIB_PROP),
+    (Crmf, ERR_LIB_CRMF),
+    (Prov, ERR_LIB_PROV),
+    (Cmp, ERR_LIB_CMP),
+    (OsslEncoder, ERR_LIB_OSSL_ENCODER),
+    (OsslDecoder, ERR_LIB_OSSL_DECODER),
+    (Http, ERR_LIB_HTTP),
+    (User, ERR_LIB_USER),
+);
+
+/// An OpenSSL error.
+pub(crate) struct Error {
+    /// The library where the error has occurred.
+    library: ErrorLibrary,
+
+    /// The reason.
+    reason: c_int,
+}
+
+impl std::fmt::Debug for Error {
+    fn fmt(&self, f: &mut std::fmt::Formatter) -> std::fmt::Result {
+        write!(
+            f,
+            "OpenSSL3Error(lib={:?}, reason={})",
+            self.library, self.reason
+        )
+    }
+}
+
+impl From<c_ulong> for Error {
+    fn from(err: c_ulong) -> Self {
+        Self {
+            library: crate::ossl3::err_get_lib(err)
+                .try_into()
+                .unwrap_or(ErrorLibrary::None),
+            reason: crate::ossl3::err_get_reason(err),
+        }
+    }
+}
+
+impl Error {
+    /// Returns the library where the error has occurred.
+    pub(crate) fn library(&self) -> ErrorLibrary {
+        self.library
+    }
+
+    /// Returns the reason of the error.
+    pub(crate) fn reason(&self) -> u32 {
+        self.reason as u32
+    }
+}
+
+gen_enum_from_openssl!(
+    SslError,
+    "SSL error",
+    (None, SSL_ERROR_NONE),
+    (Ssl, SSL_ERROR_SSL),
+    (WantRead, SSL_ERROR_WANT_READ),
+    (WantWrite, SSL_ERROR_WANT_WRITE),
+    (WantX509Lookup, SSL_ERROR_WANT_X509_LOOKUP),
+    (Syscall, SSL_ERROR_SYSCALL),
+    (ZeroReturn, SSL_ERROR_ZERO_RETURN),
+    (WantConnect, SSL_ERROR_WANT_CONNECT),
+    (WantAccept, SSL_ERROR_WANT_ACCEPT),
+    (WantAsync, SSL_ERROR_WANT_ASYNC),
+    (WantAsyncJob, SSL_ERROR_WANT_ASYNC_JOB),
+    (WantClientHelloCb, SSL_ERROR_WANT_CLIENT_HELLO_CB),
+    (WantRetryVerify, SSL_ERROR_WANT_RETRY_VERIFY),
+);
+
+impl From<SslError> for pb::RecordError {
+    fn from(ssl_error: SslError) -> Self {
+        match ssl_error {
+            SslError::WantRead => Self::RECORDERROR_WANT_READ,
+            SslError::WantWrite => Self::RECORDERROR_WANT_WRITE,
+            SslError::ZeroReturn => Self::RECORDERROR_CLOSED,
+            SslError::Syscall => match std::io::Error::last_os_error().raw_os_error() {
+                // EPIPE
+                Some(32) => Self::RECORDERROR_CLOSED,
+                _ => Self::RECORDERROR_UNKNOWN,
+            },
+            SslError::Ssl => {
+                let error = Error::from(crate::ossl3::peek_last_error());
+                if error.library() == ErrorLibrary::Ssl
+                    && error.reason() == openssl3::SSL_R_PROTOCOL_IS_SHUTDOWN
+                {
+                    Self::RECORDERROR_CLOSED
+                } else {
+                    Self::RECORDERROR_UNKNOWN
+                }
+            }
+            _ => Self::RECORDERROR_UNKNOWN,
+        }
+    }
+}
+
+
 #[cfg(test)]
-mod test {
+pub(crate) mod test {
+    use std::ffi::{c_int, CString};
+
     use super::*;
+
+    /// Flushes the current error stack.
+    fn openssl_flush_error_stack() {
+        let mut i = 20;
+        while i != 0 {
+            if unsafe { openssl3::ERR_get_error() } == 0 {
+                break;
+            }
+            i -= 1;
+        }
+        assert_ne!(i, 0);
+    }
+
+    /// Creates a new OpenSSL error.
+    fn openssl_new_error(lib: impl Into<c_int>, reason: impl Into<c_int>, msg: impl Into<String>) {
+        let lib: c_int = lib.into();
+        let reason: c_int = reason.into();
+        let msg = CString::new(msg.into()).unwrap();
+
+        unsafe {
+            openssl3::ERR_new();
+            openssl3::ERR_set_error(lib, reason, msg.as_ptr());
+        }
+    }
+
+    /// Returns a certificate ([`NativeX509Certificate`]) that has been read
+    /// from a file in the testdata directory.
+    pub(crate) fn get_certificate_from_testdata_file<'a>(
+        lib_ctx: &LibCtx<'a>,
+        path: impl AsRef<str>,
+        format: pb_api::ASN1EncodingFormat,
+    ) -> crate::Result<Pimpl<'a, NativeX509Certificate>> {
+        let path = crate::test::resolve_runfile(path.as_ref());
+        let content = std::fs::read(path).unwrap();
+        let bio = BIO_from_buffer(&content).unwrap();
+        X509_from_BIO(lib_ctx, bio.as_nonnull(), format)
+    }
+
+    /// Returns a private key ([`NativePrivateKey`]) that has been read
+    /// from a file in the testdata directory.
+    pub(crate) fn get_private_key_from_testdata_file<'a>(
+        lib_ctx: &LibCtx<'a>,
+        path: impl AsRef<str>,
+        format: pb_api::ASN1EncodingFormat,
+    ) -> crate::Result<Pimpl<'a, NativePrivateKey>> {
+        let path = crate::test::resolve_runfile(path.as_ref());
+        let content = std::fs::read(path).unwrap();
+        let bio = BIO_from_buffer(&content).unwrap();
+        EVP_PKEY_from_BIO(lib_ctx, bio.as_nonnull(), format)
+    }
+
+    /// Tests [`errstr`].
+    #[test]
+    fn test_errstr() {
+        openssl_flush_error_stack();
+        openssl_new_error(1, 2, "this is an error");
+        let result = errstr();
+
+        assert!(
+            result.contains("this is an error"),
+            "error string from OpenSSL does not seem to match the pattern defined"
+        );
+    }
+
+    /// Tests [`errstr`] with a string that matches the `DEFAULT_BUFFER_LEN`.
+    #[test]
+    fn test_errstr_default_len() {
+        let _lib_ctx = LibCtx::try_new().unwrap();
+        openssl_flush_error_stack();
+        let msg = "A".to_string().repeat(201);
+        openssl_new_error(1, 2, msg.clone());
+        let result = errstr();
+
+        assert!(
+            result.contains(&format!("error:00800002:lib(1)::reason(2)::-1:{msg}")),
+            "error string from OpenSSL does not seem to match the pattern defined"
+        );
+    }
+
+    /// Tests [`BIO_from_buffer`].
+    #[test]
+    #[allow(non_snake_case)]
+    fn test_BIO_from_buffer() {
+        let buf_in = vec![42u8; 42];
+        let bio = BIO_from_buffer(&buf_in).unwrap();
+        let mut buf_out = vec![42u8; 42];
+        let mut readbytes = 0usize;
+
+        let result = unsafe {
+            openssl3::BIO_read_ex(
+                bio.as_nonnull().as_ptr(),
+                buf_out.as_mut_ptr().cast(),
+                buf_out.len(),
+                &mut readbytes as *mut _,
+            )
+        };
+
+        assert_eq!(
+            (result, readbytes, &buf_in),
+            (1, 42, &buf_out),
+            "`BIO_read_ex` did not return the expected result"
+        );
+    }
+
+    /// Tests [`BIO_from_buffer`] with empty BIO.
+    #[test]
+    #[allow(non_snake_case)]
+    fn test_BIO_from_buffer_empty() {
+        let buf_in = vec![0u8; 0];
+        let bio = BIO_from_buffer(&buf_in).unwrap();
+        let mut buf_out = vec![0u8; 42];
+        let mut readbytes = 0usize;
+
+        let ret = unsafe {
+            openssl3::BIO_read_ex(
+                bio.as_nonnull().as_ptr(),
+                buf_out.as_mut_ptr().cast(),
+                buf_out.len(),
+                &mut readbytes as *mut _,
+            )
+        };
+
+        assert_eq!(
+            (ret, readbytes),
+            (0, 0),
+            "`BIO_read_ex` did not return 0 for an empty buffer"
+        );
+    }
+
+    /// Tests [`X509_from_BIO`] with a PEM-encoded certificate.
+    #[test]
+    #[allow(non_snake_case)]
+    fn test_X509_from_BIO_PEM() {
+        let cert_path =
+            crate::test::resolve_runfile("testdata/falcon1024.cert.pem");
+        let data = std::fs::read(cert_path).unwrap();
+        let bio = BIO_from_buffer(&data).unwrap();
+        let lib_ctx = LibCtx::try_new().unwrap();
+
+        let result = X509_from_BIO(
+            &lib_ctx,
+            bio.as_nonnull(),
+            pb_api::ASN1EncodingFormat::ENCODING_FORMAT_PEM,
+        );
+
+        result.unwrap();
+    }
+
+    /// Tests [`X509_from_BIO`] with a DER-encoded certificate.
+    #[test]
+    #[allow(non_snake_case)]
+    fn test_X509_from_BIO_DER() {
+        let cert_path =
+            crate::test::resolve_runfile("testdata/dilithium5.cert.der");
+        let data = std::fs::read(cert_path).unwrap();
+        let bio = BIO_from_buffer(&data).unwrap();
+        let lib_ctx = LibCtx::try_new().unwrap();
+
+        X509_from_BIO(
+            &lib_ctx,
+            bio.as_nonnull(),
+            pb_api::ASN1EncodingFormat::ENCODING_FORMAT_DER,
+        )
+        .unwrap();
+    }
+
+    /// Tests [`X509_from_BIO`] with an invalid DER-encoded certificate.
+    #[test]
+    #[allow(non_snake_case)]
+    fn test_X509_from_BIO_DER_invalid() {
+        let cert_path =
+            crate::test::resolve_runfile("testdata/cert_unknown_sig_alg.der");
+        let data = std::fs::read(cert_path).unwrap();
+        let bio = BIO_from_buffer(&data).unwrap();
+        let lib_ctx = LibCtx::try_new().unwrap();
+
+        let err = X509_from_BIO(
+            &lib_ctx,
+            bio.as_nonnull(),
+            pb_api::ASN1EncodingFormat::ENCODING_FORMAT_PEM,
+        );
+
+        let err = err.unwrap_err();
+        assert!(err.is(&errors! {pb::CertificateError::CERTIFICATEERROR_MALFORMED}));
+    }
+
+    /// Tests [`EVP_PKEY_from_BIO`] with a PEM-encoded private key.
+    #[test]
+    #[allow(non_snake_case)]
+    fn test_EVP_PKEY_from_BIO_PEM() {
+        let private_key_path =
+            crate::test::resolve_runfile("testdata/dilithium5.key.pem");
+        let data = std::fs::read(private_key_path).unwrap();
+        let bio = BIO_from_buffer(&data).unwrap();
+        let lib_ctx = LibCtx::try_new().unwrap();
+
+        EVP_PKEY_from_BIO(
+            &lib_ctx,
+            bio.as_nonnull(),
+            pb_api::ASN1EncodingFormat::ENCODING_FORMAT_PEM,
+        )
+        .unwrap();
+    }
+
+    /// Tests [`EVP_PKEY_from_BIO`] with a DER-encoded private key.
+    #[test]
+    #[allow(non_snake_case)]
+    fn test_EVP_PKEY_from_BIO_DER() {
+        let private_key_path =
+            crate::test::resolve_runfile("testdata/dilithium5.key.der");
+        let data = std::fs::read(private_key_path).unwrap();
+        let bio = BIO_from_buffer(&data).unwrap();
+        let lib_ctx = LibCtx::try_new().unwrap();
+
+        EVP_PKEY_from_BIO(
+            &lib_ctx,
+            bio.as_nonnull(),
+            pb_api::ASN1EncodingFormat::ENCODING_FORMAT_DER,
+        )
+        .unwrap();
+    }
+
+    /// Tests [`is_BIO_eof`].
+    #[test]
+    #[allow(non_snake_case)]
+    fn test_is_BIO_eof() {
+        let data = vec![42u8; 42];
+        let bio = BIO_from_buffer(&data).unwrap();
+        let mut buf_out = vec![42u8; 42];
+        let mut readbytes = 0usize;
+        let ret = unsafe {
+            openssl3::BIO_read_ex(
+                bio.as_nonnull().as_ptr(),
+                buf_out.as_mut_ptr().cast(),
+                buf_out.len(),
+                &mut readbytes as *mut _,
+            )
+        };
+
+        let result = is_BIO_eof(bio.as_nonnull());
+
+        assert_eq!((ret, readbytes, result), (1, buf_out.len(), true));
+    }
+
+    /// Tests [`is_BIO_eof`] with a non-empty BIO.
+    #[test]
+    #[allow(non_snake_case)]
+    fn test_is_BIO_eof_non_empty() {
+        let data = vec![42u8; 42];
+        let bio = BIO_from_buffer(&data).unwrap();
+        let mut buf_out = vec![0u8; 42];
+        let mut readbytes = 0usize;
+        let ret = unsafe {
+            openssl3::BIO_read_ex(
+                bio.as_nonnull().as_ptr(),
+                buf_out.as_mut_ptr().cast(),
+                buf_out.len() - 1,
+                &mut readbytes as *mut _,
+            )
+        };
+
+        let result = is_BIO_eof(bio.as_nonnull());
+
+        assert_eq!((ret, readbytes, result), (1, buf_out.len() - 1, false));
+    }
+
+    /// Tests [`is_BIO_eof`] with a non-empty BIO full of zeros.
+    #[test]
+    #[allow(non_snake_case)]
+    fn test_is_BIO_eof_non_empty_zeros() {
+        let data = vec![0u8; 42];
+        let bio = BIO_from_buffer(&data).unwrap();
+        let mut buf_out = vec![42u8; 42];
+        let mut readbytes = 0usize;
+        let ret = unsafe {
+            openssl3::BIO_read_ex(
+                bio.as_nonnull().as_ptr(),
+                buf_out.as_mut_ptr().cast(),
+                buf_out.len() - 1,
+                &mut readbytes as *mut _,
+            )
+        };
+
+        let result = is_BIO_eof(bio.as_nonnull());
+
+        assert_eq!((ret, readbytes, result), (1, buf_out.len() - 1, false));
+    }
 
     /// Tests [`LibCtx::try_new`].
     #[test]
