proofs/fstar/extraction/Sandwich.Implementation.Openssl3.fsti
@@ -3,13 +3,268 @@ module Sandwich.Implementation.Openssl3
 open Core
 open FStar.Mul
 
+let _ =
+  (* This module has implicit dependencies, here we make them explicit. *)
+  (* The implicit dependencies arise from typeclasses instances. *)
+  let open Sandwich.Error in
+  let open Sandwich.Error.Code in
+  let open Std.Ffi.Os_str in
+  ()
+
+let discriminant_ErrorLibrary_Asn1: isize = cast (Openssl3.v_ERR_LIB_ASN1 <: u32) <: isize
+
+let discriminant_ErrorLibrary_Async: isize = cast (Openssl3.v_ERR_LIB_ASYNC <: u32) <: isize
+
+let discriminant_ErrorLibrary_Bio: isize = cast (Openssl3.v_ERR_LIB_BIO <: u32) <: isize
+
+let discriminant_ErrorLibrary_Bn: isize = cast (Openssl3.v_ERR_LIB_BN <: u32) <: isize
+
+let discriminant_ErrorLibrary_Buf: isize = cast (Openssl3.v_ERR_LIB_BUF <: u32) <: isize
+
+let discriminant_ErrorLibrary_Cmp: isize = cast (Openssl3.v_ERR_LIB_CMP <: u32) <: isize
+
+let discriminant_ErrorLibrary_Cms: isize = cast (Openssl3.v_ERR_LIB_CMS <: u32) <: isize
+
+let discriminant_ErrorLibrary_Comp: isize = cast (Openssl3.v_ERR_LIB_COMP <: u32) <: isize
+
+let discriminant_ErrorLibrary_Conf: isize = cast (Openssl3.v_ERR_LIB_CONF <: u32) <: isize
+
+let discriminant_ErrorLibrary_Crmf: isize = cast (Openssl3.v_ERR_LIB_CRMF <: u32) <: isize
+
+let discriminant_ErrorLibrary_Crypto: isize = cast (Openssl3.v_ERR_LIB_CRYPTO <: u32) <: isize
+
+let discriminant_ErrorLibrary_Ct: isize = cast (Openssl3.v_ERR_LIB_CT <: u32) <: isize
+
+let discriminant_ErrorLibrary_Dh: isize = cast (Openssl3.v_ERR_LIB_DH <: u32) <: isize
+
+let discriminant_ErrorLibrary_Dsa: isize = cast (Openssl3.v_ERR_LIB_DSA <: u32) <: isize
+
+let discriminant_ErrorLibrary_Dso: isize = cast (Openssl3.v_ERR_LIB_DSO <: u32) <: isize
+
+let discriminant_ErrorLibrary_Ec: isize = cast (Openssl3.v_ERR_LIB_EC <: u32) <: isize
+
+let discriminant_ErrorLibrary_Ecdh: isize = cast (Openssl3.v_ERR_LIB_ECDH <: u32) <: isize
+
+let discriminant_ErrorLibrary_Ecdsa: isize = cast (Openssl3.v_ERR_LIB_ECDSA <: u32) <: isize
+
+let discriminant_ErrorLibrary_Engine: isize = cast (Openssl3.v_ERR_LIB_ENGINE <: u32) <: isize
+
+let discriminant_ErrorLibrary_Ess: isize = cast (Openssl3.v_ERR_LIB_ESS <: u32) <: isize
+
+let discriminant_ErrorLibrary_Evp: isize = cast (Openssl3.v_ERR_LIB_EVP <: u32) <: isize
+
+let discriminant_ErrorLibrary_Fips: isize = cast (Openssl3.v_ERR_LIB_FIPS <: u32) <: isize
+
+let discriminant_ErrorLibrary_Hmac: isize = cast (Openssl3.v_ERR_LIB_HMAC <: u32) <: isize
+
+let discriminant_ErrorLibrary_Http: isize = cast (Openssl3.v_ERR_LIB_HTTP <: u32) <: isize
+
+let discriminant_ErrorLibrary_Kdf: isize = cast (Openssl3.v_ERR_LIB_KDF <: u32) <: isize
+
+let discriminant_ErrorLibrary_None: isize = cast (Openssl3.v_ERR_LIB_NONE <: u32) <: isize
+
+let discriminant_ErrorLibrary_Obj: isize = cast (Openssl3.v_ERR_LIB_OBJ <: u32) <: isize
+
+let discriminant_ErrorLibrary_Ocsp: isize = cast (Openssl3.v_ERR_LIB_OCSP <: u32) <: isize
+
+let discriminant_ErrorLibrary_OsslDecoder: isize =
+  cast (Openssl3.v_ERR_LIB_OSSL_DECODER <: u32) <: isize
+
+let discriminant_ErrorLibrary_OsslEncoder: isize =
+  cast (Openssl3.v_ERR_LIB_OSSL_ENCODER <: u32) <: isize
+
+let discriminant_ErrorLibrary_OsslStore: isize =
+  cast (Openssl3.v_ERR_LIB_OSSL_STORE <: u32) <: isize
+
+let discriminant_ErrorLibrary_Pem: isize = cast (Openssl3.v_ERR_LIB_PEM <: u32) <: isize
+
+let discriminant_ErrorLibrary_Pkcs12: isize = cast (Openssl3.v_ERR_LIB_PKCS12 <: u32) <: isize
+
+let discriminant_ErrorLibrary_Pkcs7: isize = cast (Openssl3.v_ERR_LIB_PKCS7 <: u32) <: isize
+
+let discriminant_ErrorLibrary_Prop: isize = cast (Openssl3.v_ERR_LIB_PROP <: u32) <: isize
+
+let discriminant_ErrorLibrary_Prov: isize = cast (Openssl3.v_ERR_LIB_PROV <: u32) <: isize
+
+let discriminant_ErrorLibrary_Rand: isize = cast (Openssl3.v_ERR_LIB_RAND <: u32) <: isize
+
+let discriminant_ErrorLibrary_Rsa: isize = cast (Openssl3.v_ERR_LIB_RSA <: u32) <: isize
+
+let discriminant_ErrorLibrary_Sm2: isize = cast (Openssl3.v_ERR_LIB_SM2 <: u32) <: isize
+
+let discriminant_ErrorLibrary_Ssl: isize = cast (Openssl3.v_ERR_LIB_SSL <: u32) <: isize
+
+let discriminant_ErrorLibrary_Sys: isize = cast (Openssl3.v_ERR_LIB_SYS <: u32) <: isize
+
+let discriminant_ErrorLibrary_Ts: isize = cast (Openssl3.v_ERR_LIB_TS <: u32) <: isize
+
+let discriminant_ErrorLibrary_Ui: isize = cast (Openssl3.v_ERR_LIB_UI <: u32) <: isize
+
+let discriminant_ErrorLibrary_User: isize = cast (Openssl3.v_ERR_LIB_USER <: u32) <: isize
+
+let discriminant_ErrorLibrary_X509: isize = cast (Openssl3.v_ERR_LIB_X509 <: u32) <: isize
+
+///Library where an error can occur
+type t_ErrorLibrary =
+  | ErrorLibrary_None : t_ErrorLibrary
+  | ErrorLibrary_Sys : t_ErrorLibrary
+  | ErrorLibrary_Bn : t_ErrorLibrary
+  | ErrorLibrary_Rsa : t_ErrorLibrary
+  | ErrorLibrary_Dh : t_ErrorLibrary
+  | ErrorLibrary_Evp : t_ErrorLibrary
+  | ErrorLibrary_Buf : t_ErrorLibrary
+  | ErrorLibrary_Obj : t_ErrorLibrary
+  | ErrorLibrary_Pem : t_ErrorLibrary
+  | ErrorLibrary_Dsa : t_ErrorLibrary
+  | ErrorLibrary_X509 : t_ErrorLibrary
+  | ErrorLibrary_Asn1 : t_ErrorLibrary
+  | ErrorLibrary_Conf : t_ErrorLibrary
+  | ErrorLibrary_Crypto : t_ErrorLibrary
+  | ErrorLibrary_Ec : t_ErrorLibrary
+  | ErrorLibrary_Ssl : t_ErrorLibrary
+  | ErrorLibrary_Bio : t_ErrorLibrary
+  | ErrorLibrary_Pkcs7 : t_ErrorLibrary
+  | ErrorLibrary_X509v3 : t_ErrorLibrary
+  | ErrorLibrary_Pkcs12 : t_ErrorLibrary
+  | ErrorLibrary_Rand : t_ErrorLibrary
+  | ErrorLibrary_Dso : t_ErrorLibrary
+  | ErrorLibrary_Engine : t_ErrorLibrary
+  | ErrorLibrary_Ocsp : t_ErrorLibrary
+  | ErrorLibrary_Ui : t_ErrorLibrary
+  | ErrorLibrary_Comp : t_ErrorLibrary
+  | ErrorLibrary_Ecdsa : t_ErrorLibrary
+  | ErrorLibrary_Ecdh : t_ErrorLibrary
+  | ErrorLibrary_OsslStore : t_ErrorLibrary
+  | ErrorLibrary_Fips : t_ErrorLibrary
+  | ErrorLibrary_Cms : t_ErrorLibrary
+  | ErrorLibrary_Ts : t_ErrorLibrary
+  | ErrorLibrary_Hmac : t_ErrorLibrary
+  | ErrorLibrary_Ct : t_ErrorLibrary
+  | ErrorLibrary_Async : t_ErrorLibrary
+  | ErrorLibrary_Kdf : t_ErrorLibrary
+  | ErrorLibrary_Sm2 : t_ErrorLibrary
+  | ErrorLibrary_Ess : t_ErrorLibrary
+  | ErrorLibrary_Prop : t_ErrorLibrary
+  | ErrorLibrary_Crmf : t_ErrorLibrary
+  | ErrorLibrary_Prov : t_ErrorLibrary
+  | ErrorLibrary_Cmp : t_ErrorLibrary
+  | ErrorLibrary_OsslEncoder : t_ErrorLibrary
+  | ErrorLibrary_OsslDecoder : t_ErrorLibrary
+  | ErrorLibrary_Http : t_ErrorLibrary
+  | ErrorLibrary_User : t_ErrorLibrary
+
+let discriminant_ErrorLibrary_X509v3: isize = cast (Openssl3.v_ERR_LIB_X509V3 <: u32) <: isize
+
+val t_ErrorLibrary_cast_to_repr (x: t_ErrorLibrary)
+    : Prims.Pure isize Prims.l_True (fun _ -> Prims.l_True)
+
+/// Sets the library context.
+val impl__ProviderBuilder__lib_ctx
+      (self: t_ProviderBuilder)
+      (lib_ctx: Core.Ptr.Non_null.t_NonNull Openssl3.t_ossl_lib_ctx_st)
+    : Prims.Pure t_ProviderBuilder Prims.l_True (fun _ -> Prims.l_True)
+
+(* item error backend: (reject_RawOrMutPointer) ExplicitRejection { reason: "a node of kind [Raw_pointer] have been found in the AST" }
+Last available AST for this item:
+
+/// Sets the name.
+#[cfg(feature = "openssl3")]
+#[deny(bare_trait_objects)]
+#[feature(register_tool)]
+#[register_tool(_hax)]
+fn impl__ProviderBuilder__name(
+    self: sandwich::implementation::openssl3::t_ProviderBuilder,
+    name: raw_pointer!(),
+) -> sandwich::implementation::openssl3::t_ProviderBuilder {
+    {
+        sandwich::implementation::openssl3::ProviderBuilder {
+            f_name: core::option::Option_Some(name),
+            ..(self)
+        }
+    }
+}
+
+
+Last AST:
+/** print_rust: pitem: not implemented  (item: { Concrete_ident.T.def_id =
+  { Concrete_ident.Imported.krate = "sandwich";
+    path =
+    [{ Concrete_ident.Imported.data =
+       (Concrete_ident.Imported.TypeNs "implementation"); disambiguator = 0 };
+      { Concrete_ident.Imported.data =
+        (Concrete_ident.Imported.TypeNs "openssl3"); disambiguator = 0 };
+      { Concrete_ident.Imported.data = Concrete_ident.Imported.Impl;
+        disambiguator = 1 };
+      { Concrete_ident.Imported.data =
+        (Concrete_ident.Imported.ValueNs "name"); disambiguator = 0 }
+      ]
+    };
+  kind = Concrete_ident.Kind.Value }) */
+const _: () = ();
+ *)
+
+/// Initializes a builder.
+val impl__ProviderBuilder__new: Prims.unit
+  -> Prims.Pure t_ProviderBuilder Prims.l_True (fun _ -> Prims.l_True)
+
 [@@ FStar.Tactics.Typeclasses.tcinstance]
-let impl_1: Core.Default.t_Default t_ProviderBuilder =
+let impl: Core.Default.t_Default t_ProviderBuilder =
   {
     f_default_pre = (fun (_: Prims.unit) -> true);
     f_default_post = (fun (_: Prims.unit) (out: t_ProviderBuilder) -> true);
     f_default = fun (_: Prims.unit) -> impl__ProviderBuilder__new ()
   }
+
+let discriminant_SslError_None: isize = cast (Openssl3.v_SSL_ERROR_NONE <: u32) <: isize
+
+let discriminant_SslError_Ssl: isize = cast (Openssl3.v_SSL_ERROR_SSL <: u32) <: isize
+
+let discriminant_SslError_Syscall: isize = cast (Openssl3.v_SSL_ERROR_SYSCALL <: u32) <: isize
+
+let discriminant_SslError_WantAccept: isize =
+  cast (Openssl3.v_SSL_ERROR_WANT_ACCEPT <: u32) <: isize
+
+let discriminant_SslError_WantAsync: isize = cast (Openssl3.v_SSL_ERROR_WANT_ASYNC <: u32) <: isize
+
+let discriminant_SslError_WantAsyncJob: isize =
+  cast (Openssl3.v_SSL_ERROR_WANT_ASYNC_JOB <: u32) <: isize
+
+let discriminant_SslError_WantClientHelloCb: isize =
+  cast (Openssl3.v_SSL_ERROR_WANT_CLIENT_HELLO_CB <: u32) <: isize
+
+let discriminant_SslError_WantConnect: isize =
+  cast (Openssl3.v_SSL_ERROR_WANT_CONNECT <: u32) <: isize
+
+let discriminant_SslError_WantRead: isize = cast (Openssl3.v_SSL_ERROR_WANT_READ <: u32) <: isize
+
+let discriminant_SslError_WantRetryVerify: isize =
+  cast (Openssl3.v_SSL_ERROR_WANT_RETRY_VERIFY <: u32) <: isize
+
+let discriminant_SslError_WantWrite: isize = cast (Openssl3.v_SSL_ERROR_WANT_WRITE <: u32) <: isize
+
+let discriminant_SslError_WantX509Lookup: isize =
+  cast (Openssl3.v_SSL_ERROR_WANT_X509_LOOKUP <: u32) <: isize
+
+///SSL error
+type t_SslError =
+  | SslError_None : t_SslError
+  | SslError_Ssl : t_SslError
+  | SslError_WantRead : t_SslError
+  | SslError_WantWrite : t_SslError
+  | SslError_WantX509Lookup : t_SslError
+  | SslError_Syscall : t_SslError
+  | SslError_ZeroReturn : t_SslError
+  | SslError_WantConnect : t_SslError
+  | SslError_WantAccept : t_SslError
+  | SslError_WantAsync : t_SslError
+  | SslError_WantAsyncJob : t_SslError
+  | SslError_WantClientHelloCb : t_SslError
+  | SslError_WantRetryVerify : t_SslError
+
+let discriminant_SslError_ZeroReturn: isize =
+  cast (Openssl3.v_SSL_ERROR_ZERO_RETURN <: u32) <: isize
+
+val t_SslError_cast_to_repr (x: t_SslError) : Prims.Pure isize Prims.l_True (fun _ -> Prims.l_True)
 
 /// The default provider name.
 let v_DEFAULT_PROVIDER_NAME: t_Array u8 (sz 8) =
@@ -23,43 +278,333 @@ let v_OQS_PROVIDER_NAME: t_Array u8 (sz 12) =
   FStar.Pervasives.assert_norm (Prims.eq2 (List.Tot.length list) 12);
   Rust_primitives.Hax.array_of_list 12 list
 
-/// A wrapper around an `OSSL_PROVIDER`.
-type t_Provider =
-  | Provider : Sandwich.Support.Pimpl.t_Pimpl Openssl3.t_ossl_provider_st -> t_Provider
+/// Returns the cipher name in the OpenSSL format.
+val cipher_name
+      (#impl_488124255_: Type0)
+      {| i1: Core.Convert.t_AsRef impl_488124255_ string |}
+      (name: impl_488124255_)
+    : Prims.Pure (Core.Option.t_Option string) Prims.l_True (fun _ -> Prims.l_True)
+
+/// Returns the library where a given error occurred.
+/// This function reproduces the `ERR_GET_LIB` method from OpenSSL, which
+/// is a static function in header (thus not understandable by bindgen).
+val err_get_lib (err: u64) : Prims.Pure i32 Prims.l_True (fun _ -> Prims.l_True)
+
+/// Returns the reason of why a given error occurred.
+/// This function reproduces the `ERR_GET_REASON` method from OpenSSL, which
+/// is a static function in header (thus not understandable by bindgen).
+val err_get_reason (err: u64) : Prims.Pure i32 Prims.l_True (fun _ -> Prims.l_True)
+
+let errstr__DEFAULT_BUFFER_LEN: usize = sz 256
+
+/// Tells if a BIO has reached EOF.
+val is_BIO_eof (bio: Core.Ptr.Non_null.t_NonNull Openssl3.t_bio_st)
+    : Prims.Pure bool Prims.l_True (fun _ -> Prims.l_True)
+
+/// Returns the last error.
+val peek_last_error: Prims.unit -> Prims.Pure u64 Prims.l_True (fun _ -> Prims.l_True)
 
 [@@ FStar.Tactics.Typeclasses.tcinstance]
-let impl: Core.Fmt.t_Debug t_Provider =
+let impl_8: Core.Convert.t_TryFrom t_ErrorLibrary i32 =
   {
-    f_fmt_pre = (fun (self: t_Provider) (f: Core.Fmt.t_Formatter) -> true);
+    f_Error = Prims.unit;
+    f_try_from_pre = (fun (err: i32) -> true);
+    f_try_from_post = (fun (err: i32) (out: Core.Result.t_Result t_ErrorLibrary Prims.unit) -> true);
+    f_try_from
+    =
+    fun (err: i32) ->
+      match cast (err <: i32) <: u32 with
+      | 1ul ->
+        Core.Result.Result_Ok (ErrorLibrary_None <: t_ErrorLibrary)
+        <:
+        Core.Result.t_Result t_ErrorLibrary Prims.unit
+      | 2ul ->
+        Core.Result.Result_Ok (ErrorLibrary_Sys <: t_ErrorLibrary)
+        <:
+        Core.Result.t_Result t_ErrorLibrary Prims.unit
+      | 3ul ->
+        Core.Result.Result_Ok (ErrorLibrary_Bn <: t_ErrorLibrary)
+        <:
+        Core.Result.t_Result t_ErrorLibrary Prims.unit
+      | 4ul ->
+        Core.Result.Result_Ok (ErrorLibrary_Rsa <: t_ErrorLibrary)
+        <:
+        Core.Result.t_Result t_ErrorLibrary Prims.unit
+      | 5ul ->
+        Core.Result.Result_Ok (ErrorLibrary_Dh <: t_ErrorLibrary)
+        <:
+        Core.Result.t_Result t_ErrorLibrary Prims.unit
+      | 6ul ->
+        Core.Result.Result_Ok (ErrorLibrary_Evp <: t_ErrorLibrary)
+        <:
+        Core.Result.t_Result t_ErrorLibrary Prims.unit
+      | 7ul ->
+        Core.Result.Result_Ok (ErrorLibrary_Buf <: t_ErrorLibrary)
+        <:
+        Core.Result.t_Result t_ErrorLibrary Prims.unit
+      | 8ul ->
+        Core.Result.Result_Ok (ErrorLibrary_Obj <: t_ErrorLibrary)
+        <:
+        Core.Result.t_Result t_ErrorLibrary Prims.unit
+      | 9ul ->
+        Core.Result.Result_Ok (ErrorLibrary_Pem <: t_ErrorLibrary)
+        <:
+        Core.Result.t_Result t_ErrorLibrary Prims.unit
+      | 10ul ->
+        Core.Result.Result_Ok (ErrorLibrary_Dsa <: t_ErrorLibrary)
+        <:
+        Core.Result.t_Result t_ErrorLibrary Prims.unit
+      | 11ul ->
+        Core.Result.Result_Ok (ErrorLibrary_X509 <: t_ErrorLibrary)
+        <:
+        Core.Result.t_Result t_ErrorLibrary Prims.unit
+      | 13ul ->
+        Core.Result.Result_Ok (ErrorLibrary_Asn1 <: t_ErrorLibrary)
+        <:
+        Core.Result.t_Result t_ErrorLibrary Prims.unit
+      | 14ul ->
+        Core.Result.Result_Ok (ErrorLibrary_Conf <: t_ErrorLibrary)
+        <:
+        Core.Result.t_Result t_ErrorLibrary Prims.unit
+      | 15ul ->
+        Core.Result.Result_Ok (ErrorLibrary_Crypto <: t_ErrorLibrary)
+        <:
+        Core.Result.t_Result t_ErrorLibrary Prims.unit
+      | 16ul ->
+        Core.Result.Result_Ok (ErrorLibrary_Ec <: t_ErrorLibrary)
+        <:
+        Core.Result.t_Result t_ErrorLibrary Prims.unit
+      | 20ul ->
+        Core.Result.Result_Ok (ErrorLibrary_Ssl <: t_ErrorLibrary)
+        <:
+        Core.Result.t_Result t_ErrorLibrary Prims.unit
+      | 32ul ->
+        Core.Result.Result_Ok (ErrorLibrary_Bio <: t_ErrorLibrary)
+        <:
+        Core.Result.t_Result t_ErrorLibrary Prims.unit
+      | 33ul ->
+        Core.Result.Result_Ok (ErrorLibrary_Pkcs7 <: t_ErrorLibrary)
+        <:
+        Core.Result.t_Result t_ErrorLibrary Prims.unit
+      | 34ul ->
+        Core.Result.Result_Ok (ErrorLibrary_X509v3 <: t_ErrorLibrary)
+        <:
+        Core.Result.t_Result t_ErrorLibrary Prims.unit
+      | 35ul ->
+        Core.Result.Result_Ok (ErrorLibrary_Pkcs12 <: t_ErrorLibrary)
+        <:
+        Core.Result.t_Result t_ErrorLibrary Prims.unit
+      | 36ul ->
+        Core.Result.Result_Ok (ErrorLibrary_Rand <: t_ErrorLibrary)
+        <:
+        Core.Result.t_Result t_ErrorLibrary Prims.unit
+      | 37ul ->
+        Core.Result.Result_Ok (ErrorLibrary_Dso <: t_ErrorLibrary)
+        <:
+        Core.Result.t_Result t_ErrorLibrary Prims.unit
+      | 38ul ->
+        Core.Result.Result_Ok (ErrorLibrary_Engine <: t_ErrorLibrary)
+        <:
+        Core.Result.t_Result t_ErrorLibrary Prims.unit
+      | 39ul ->
+        Core.Result.Result_Ok (ErrorLibrary_Ocsp <: t_ErrorLibrary)
+        <:
+        Core.Result.t_Result t_ErrorLibrary Prims.unit
+      | 40ul ->
+        Core.Result.Result_Ok (ErrorLibrary_Ui <: t_ErrorLibrary)
+        <:
+        Core.Result.t_Result t_ErrorLibrary Prims.unit
+      | 41ul ->
+        Core.Result.Result_Ok (ErrorLibrary_Comp <: t_ErrorLibrary)
+        <:
+        Core.Result.t_Result t_ErrorLibrary Prims.unit
+      | 42ul ->
+        Core.Result.Result_Ok (ErrorLibrary_Ecdsa <: t_ErrorLibrary)
+        <:
+        Core.Result.t_Result t_ErrorLibrary Prims.unit
+      | 43ul ->
+        Core.Result.Result_Ok (ErrorLibrary_Ecdh <: t_ErrorLibrary)
+        <:
+        Core.Result.t_Result t_ErrorLibrary Prims.unit
+      | 44ul ->
+        Core.Result.Result_Ok (ErrorLibrary_OsslStore <: t_ErrorLibrary)
+        <:
+        Core.Result.t_Result t_ErrorLibrary Prims.unit
+      | 45ul ->
+        Core.Result.Result_Ok (ErrorLibrary_Fips <: t_ErrorLibrary)
+        <:
+        Core.Result.t_Result t_ErrorLibrary Prims.unit
+      | 46ul ->
+        Core.Result.Result_Ok (ErrorLibrary_Cms <: t_ErrorLibrary)
+        <:
+        Core.Result.t_Result t_ErrorLibrary Prims.unit
+      | 47ul ->
+        Core.Result.Result_Ok (ErrorLibrary_Ts <: t_ErrorLibrary)
+        <:
+        Core.Result.t_Result t_ErrorLibrary Prims.unit
+      | 48ul ->
+        Core.Result.Result_Ok (ErrorLibrary_Hmac <: t_ErrorLibrary)
+        <:
+        Core.Result.t_Result t_ErrorLibrary Prims.unit
+      | 50ul ->
+        Core.Result.Result_Ok (ErrorLibrary_Ct <: t_ErrorLibrary)
+        <:
+        Core.Result.t_Result t_ErrorLibrary Prims.unit
+      | 51ul ->
+        Core.Result.Result_Ok (ErrorLibrary_Async <: t_ErrorLibrary)
+        <:
+        Core.Result.t_Result t_ErrorLibrary Prims.unit
+      | 52ul ->
+        Core.Result.Result_Ok (ErrorLibrary_Kdf <: t_ErrorLibrary)
+        <:
+        Core.Result.t_Result t_ErrorLibrary Prims.unit
+      | 53ul ->
+        Core.Result.Result_Ok (ErrorLibrary_Sm2 <: t_ErrorLibrary)
+        <:
+        Core.Result.t_Result t_ErrorLibrary Prims.unit
+      | 54ul ->
+        Core.Result.Result_Ok (ErrorLibrary_Ess <: t_ErrorLibrary)
+        <:
+        Core.Result.t_Result t_ErrorLibrary Prims.unit
+      | 55ul ->
+        Core.Result.Result_Ok (ErrorLibrary_Prop <: t_ErrorLibrary)
+        <:
+        Core.Result.t_Result t_ErrorLibrary Prims.unit
+      | 56ul ->
+        Core.Result.Result_Ok (ErrorLibrary_Crmf <: t_ErrorLibrary)
+        <:
+        Core.Result.t_Result t_ErrorLibrary Prims.unit
+      | 57ul ->
+        Core.Result.Result_Ok (ErrorLibrary_Prov <: t_ErrorLibrary)
+        <:
+        Core.Result.t_Result t_ErrorLibrary Prims.unit
+      | 58ul ->
+        Core.Result.Result_Ok (ErrorLibrary_Cmp <: t_ErrorLibrary)
+        <:
+        Core.Result.t_Result t_ErrorLibrary Prims.unit
+      | 59ul ->
+        Core.Result.Result_Ok (ErrorLibrary_OsslEncoder <: t_ErrorLibrary)
+        <:
+        Core.Result.t_Result t_ErrorLibrary Prims.unit
+      | 60ul ->
+        Core.Result.Result_Ok (ErrorLibrary_OsslDecoder <: t_ErrorLibrary)
+        <:
+        Core.Result.t_Result t_ErrorLibrary Prims.unit
+      | 61ul ->
+        Core.Result.Result_Ok (ErrorLibrary_Http <: t_ErrorLibrary)
+        <:
+        Core.Result.t_Result t_ErrorLibrary Prims.unit
+      | 128ul ->
+        Core.Result.Result_Ok (ErrorLibrary_User <: t_ErrorLibrary)
+        <:
+        Core.Result.t_Result t_ErrorLibrary Prims.unit
+      | _ ->
+        Core.Result.Result_Err (() <: Prims.unit) <: Core.Result.t_Result t_ErrorLibrary Prims.unit
+  }
+
+[@@ FStar.Tactics.Typeclasses.tcinstance]
+let impl_15: Core.Convert.t_TryFrom t_SslError i32 =
+  {
+    f_Error = Prims.unit;
+    f_try_from_pre = (fun (err: i32) -> true);
+    f_try_from_post = (fun (err: i32) (out: Core.Result.t_Result t_SslError Prims.unit) -> true);
+    f_try_from
+    =
+    fun (err: i32) ->
+      match cast (err <: i32) <: u32 with
+      | 0ul ->
+        Core.Result.Result_Ok (SslError_None <: t_SslError)
+        <:
+        Core.Result.t_Result t_SslError Prims.unit
+      | 1ul ->
+        Core.Result.Result_Ok (SslError_Ssl <: t_SslError)
+        <:
+        Core.Result.t_Result t_SslError Prims.unit
+      | 2ul ->
+        Core.Result.Result_Ok (SslError_WantRead <: t_SslError)
+        <:
+        Core.Result.t_Result t_SslError Prims.unit
+      | 3ul ->
+        Core.Result.Result_Ok (SslError_WantWrite <: t_SslError)
+        <:
+        Core.Result.t_Result t_SslError Prims.unit
+      | 4ul ->
+        Core.Result.Result_Ok (SslError_WantX509Lookup <: t_SslError)
+        <:
+        Core.Result.t_Result t_SslError Prims.unit
+      | 5ul ->
+        Core.Result.Result_Ok (SslError_Syscall <: t_SslError)
+        <:
+        Core.Result.t_Result t_SslError Prims.unit
+      | 6ul ->
+        Core.Result.Result_Ok (SslError_ZeroReturn <: t_SslError)
+        <:
+        Core.Result.t_Result t_SslError Prims.unit
+      | 7ul ->
+        Core.Result.Result_Ok (SslError_WantConnect <: t_SslError)
+        <:
+        Core.Result.t_Result t_SslError Prims.unit
+      | 8ul ->
+        Core.Result.Result_Ok (SslError_WantAccept <: t_SslError)
+        <:
+        Core.Result.t_Result t_SslError Prims.unit
+      | 9ul ->
+        Core.Result.Result_Ok (SslError_WantAsync <: t_SslError)
+        <:
+        Core.Result.t_Result t_SslError Prims.unit
+      | 10ul ->
+        Core.Result.Result_Ok (SslError_WantAsyncJob <: t_SslError)
+        <:
+        Core.Result.t_Result t_SslError Prims.unit
+      | 11ul ->
+        Core.Result.Result_Ok (SslError_WantClientHelloCb <: t_SslError)
+        <:
+        Core.Result.t_Result t_SslError Prims.unit
+      | 12ul ->
+        Core.Result.Result_Ok (SslError_WantRetryVerify <: t_SslError)
+        <:
+        Core.Result.t_Result t_SslError Prims.unit
+      | _ -> Core.Result.Result_Err (() <: Prims.unit) <: Core.Result.t_Result t_SslError Prims.unit
+  }
+
+/// An OpenSSL error.
+type t_Error = {
+  f_library:t_ErrorLibrary;
+  f_reason:i32
+}
+
+[@@ FStar.Tactics.Typeclasses.tcinstance]
+let impl_3: Core.Fmt.t_Debug t_Error =
+  {
+    f_fmt_pre = (fun (self: t_Error) (f: Core.Fmt.t_Formatter) -> true);
     f_fmt_post
     =
     (fun
-        (self: t_Provider)
+        (self: t_Error)
         (f: Core.Fmt.t_Formatter)
         (out1: (Core.Fmt.t_Formatter & Core.Result.t_Result Prims.unit Core.Fmt.t_Error))
         ->
         true);
     f_fmt
     =
-    fun (self: t_Provider) (f: Core.Fmt.t_Formatter) ->
+    fun (self: t_Error) (f: Core.Fmt.t_Formatter) ->
       let tmp0, out:(Core.Fmt.t_Formatter & Core.Result.t_Result Prims.unit Core.Fmt.t_Error) =
         Core.Fmt.impl_7__write_fmt f
-          (Core.Fmt.impl_2__new_v1 (sz 1)
-              (sz 1)
-              (let list = ["Provider("] in
-                FStar.Pervasives.assert_norm (Prims.eq2 (List.Tot.length list) 1);
-                Rust_primitives.Hax.array_of_list 1 list)
+          (Core.Fmt.impl_2__new_v1 (sz 3)
+              (sz 2)
+              (let list = ["OpenSSL3Error(lib="; ", reason="; ")"] in
+                FStar.Pervasives.assert_norm (Prims.eq2 (List.Tot.length list) 3);
+                Rust_primitives.Hax.array_of_list 3 list)
               (let list =
                   [
-                    Rust_primitives.Hax.failure "(reject_RawOrMutPointer) ExplicitRejection { reason: \"a node of kind [Raw_pointer] have been found in the AST\" }"
-                      "core::fmt::rt::impl_1__new_pointer::<\n        lifetime!(something),\n        raw_pointer!(),\n    >(\n        &(deref(\n            &(core::ptr::non_null::impl_3__as_ptr::<\n                openssl3::t_ossl_provider_st,\n            >(\n                sandwich::support::pimpl::impl_2__as_nonnull::<\n                    lifetime!(something),\n                    openssl3::t_ossl_provider_st,\n                >(&(proj_sandwich::implementation::openssl3::_0(deref(self)))),\n            )),\n        )),\n    )"
-
+                    Core.Fmt.Rt.impl_1__new_debug #t_ErrorLibrary self.f_library
                     <:
-                    Core.Fmt.Rt.t_Argument
+                    Core.Fmt.Rt.t_Argument;
+                    Core.Fmt.Rt.impl_1__new_display #i32 self.f_reason <: Core.Fmt.Rt.t_Argument
                   ]
                 in
-                FStar.Pervasives.assert_norm (Prims.eq2 (List.Tot.length list) 1);
-                Rust_primitives.Hax.array_of_list 1 list)
+                FStar.Pervasives.assert_norm (Prims.eq2 (List.Tot.length list) 2);
+                Rust_primitives.Hax.array_of_list 2 list)
             <:
             Core.Fmt.t_Arguments)
       in
@@ -70,9 +615,157 @@ let impl: Core.Fmt.t_Debug t_Provider =
       (Core.Fmt.t_Formatter & Core.Result.t_Result Prims.unit Core.Fmt.t_Error)
   }
 
+[@@ FStar.Tactics.Typeclasses.tcinstance]
+let impl_4: Core.Convert.t_From t_Error u64 =
+  {
+    f_from_pre = (fun (err: u64) -> true);
+    f_from_post = (fun (err: u64) (out: t_Error) -> true);
+    f_from
+    =
+    fun (err: u64) ->
+      {
+        f_library
+        =
+        Core.Result.impl__unwrap_or #t_ErrorLibrary
+          #Prims.unit
+          (Core.Convert.f_try_into #i32
+              #t_ErrorLibrary
+              #FStar.Tactics.Typeclasses.solve
+              (err_get_lib err <: i32)
+            <:
+            Core.Result.t_Result t_ErrorLibrary Prims.unit)
+          (ErrorLibrary_None <: t_ErrorLibrary);
+        f_reason = err_get_reason err
+      }
+      <:
+      t_Error
+  }
+
+/// Returns the library where the error has occurred.
+val impl__Error__library (self: t_Error)
+    : Prims.Pure t_ErrorLibrary Prims.l_True (fun _ -> Prims.l_True)
+
+/// Returns the reason of the error.
+val impl__Error__reason (self: t_Error) : Prims.Pure u32 Prims.l_True (fun _ -> Prims.l_True)
+
+[@@ FStar.Tactics.Typeclasses.tcinstance]
+let impl_6: Core.Convert.t_From Sandwich_proto.Tunnel.t_RecordError t_SslError =
+  {
+    f_from_pre = (fun (ssl_error: t_SslError) -> true);
+    f_from_post = (fun (ssl_error: t_SslError) (out: Sandwich_proto.Tunnel.t_RecordError) -> true);
+    f_from
+    =
+    fun (ssl_error: t_SslError) ->
+      match ssl_error with
+      | SslError_WantRead  ->
+        Sandwich_proto.Tunnel.RecordError_RECORDERROR_WANT_READ
+        <:
+        Sandwich_proto.Tunnel.t_RecordError
+      | SslError_WantWrite  ->
+        Sandwich_proto.Tunnel.RecordError_RECORDERROR_WANT_WRITE
+        <:
+        Sandwich_proto.Tunnel.t_RecordError
+      | SslError_ZeroReturn  ->
+        Sandwich_proto.Tunnel.RecordError_RECORDERROR_CLOSED <: Sandwich_proto.Tunnel.t_RecordError
+      | SslError_Syscall  ->
+        (match
+            Std.Io.Error.impl__Error__raw_os_error (Std.Io.Error.impl__Error__last_os_error ()
+                <:
+                Std.Io.Error.t_Error)
+          with
+          | Core.Option.Option_Some 32l ->
+            Sandwich_proto.Tunnel.RecordError_RECORDERROR_CLOSED
+            <:
+            Sandwich_proto.Tunnel.t_RecordError
+          | _ ->
+            Sandwich_proto.Tunnel.RecordError_RECORDERROR_UNKNOWN
+            <:
+            Sandwich_proto.Tunnel.t_RecordError)
+      | SslError_Ssl  ->
+        let error:t_Error =
+          Core.Convert.f_from #t_Error
+            #u64
+            #FStar.Tactics.Typeclasses.solve
+            (peek_last_error () <: u64)
+        in
+        if
+          (impl__Error__library error <: t_ErrorLibrary) =. (ErrorLibrary_Ssl <: t_ErrorLibrary) &&
+          (impl__Error__reason error <: u32) =. Openssl3.v_SSL_R_PROTOCOL_IS_SHUTDOWN
+        then
+          Sandwich_proto.Tunnel.RecordError_RECORDERROR_CLOSED
+          <:
+          Sandwich_proto.Tunnel.t_RecordError
+        else
+          Sandwich_proto.Tunnel.RecordError_RECORDERROR_UNKNOWN
+          <:
+          Sandwich_proto.Tunnel.t_RecordError
+      | _ ->
+        Sandwich_proto.Tunnel.RecordError_RECORDERROR_UNKNOWN <: Sandwich_proto.Tunnel.t_RecordError
+  }
+
+/// Returns a string containing the error strings for all errors that
+/// OpenSSL 3 has recorded.
+/// This function clears the error queue.
+val errstr: Prims.unit -> Prims.Pure Alloc.String.t_String Prims.l_True (fun _ -> Prims.l_True)
+
+/// A wrapper around an `OSSL_PROVIDER`.
+type t_Provider =
+  | Provider : Sandwich.Support.Pimpl.t_Pimpl Openssl3.t_ossl_provider_st -> t_Provider
+
+/// Builds the provider.
+val impl__ProviderBuilder__build (self: t_ProviderBuilder)
+    : Prims.Pure (Core.Result.t_Result t_Provider Sandwich.Error.t_Error)
+      Prims.l_True
+      (fun _ -> Prims.l_True)
+
+/// Creates a `BIO` object from a immutable buffer.
+val v_BIO_from_buffer
+      (#impl_424714745_: Type0)
+      {| i1: Core.Convert.t_AsRef impl_424714745_ (t_Slice u8) |}
+      (buffer: impl_424714745_)
+    : Prims.Pure
+      (Core.Result.t_Result (Sandwich.Support.Pimpl.t_Pimpl Openssl3.t_bio_st)
+          Sandwich.Error.t_Error) Prims.l_True (fun _ -> Prims.l_True)
+
+/// Creates a new `BIO` object with a specific method.
+val new_BIO (bio_meth: Core.Ptr.Non_null.t_NonNull Openssl3.t_bio_method_st)
+    : Prims.Pure
+      (Core.Result.t_Result (Sandwich.Support.Pimpl.t_Pimpl Openssl3.t_bio_st)
+          Sandwich.Error.t_Error) Prims.l_True (fun _ -> Prims.l_True)
+
 /// An `OSSL_LIB_CTX` object wrapped in a `Pimpl`.
 type t_LibCtx = {
   f__oqs_provider:t_Provider;
   f__default_provider:t_Provider;
   f_lib_ctx:Sandwich.Support.Pimpl.t_Pimpl Openssl3.t_ossl_lib_ctx_st
 }
+
+/// Returns a pointer to the top-level library context.
+val impl_2__as_nonnull (self: t_LibCtx)
+    : Prims.Pure (Core.Ptr.Non_null.t_NonNull Openssl3.t_ossl_lib_ctx_st)
+      Prims.l_True
+      (fun _ -> Prims.l_True)
+
+/// Instantiates a new top-level library context.
+val impl_2__try_new: Prims.unit
+  -> Prims.Pure (Core.Result.t_Result t_LibCtx Sandwich.Error.t_Error)
+      Prims.l_True
+      (fun _ -> Prims.l_True)
+
+/// Reads a private key (`EVP_PKEY` object) from a `BIO` object.
+val v_EVP_PKEY_from_BIO
+      (lib_ctx: t_LibCtx)
+      (bio: Core.Ptr.Non_null.t_NonNull Openssl3.t_bio_st)
+      (format: Sandwich_api_proto.Encoding_format.t_ASN1EncodingFormat)
+    : Prims.Pure
+      (Core.Result.t_Result (Sandwich.Support.Pimpl.t_Pimpl Openssl3.t_evp_pkey_st)
+          Sandwich.Error.t_Error) Prims.l_True (fun _ -> Prims.l_True)
+
+/// Reads a certificate (`X509` object) from a `BIO` object.
+val v_X509_from_BIO
+      (lib_ctx: t_LibCtx)
+      (bio: Core.Ptr.Non_null.t_NonNull Openssl3.t_bio_st)
+      (format: Sandwich_api_proto.Encoding_format.t_ASN1EncodingFormat)
+    : Prims.Pure
+      (Core.Result.t_Result (Sandwich.Support.Pimpl.t_Pimpl Openssl3.t_x509_st)
+          Sandwich.Error.t_Error) Prims.l_True (fun _ -> Prims.l_True)
