proofs/fstar/extraction/Sandwich.Implementation.Openssl3.Support.fsti
@@ -1,0 +1,75 @@
+module Sandwich.Implementation.Openssl3.Support
+#set-options "--fuel 0 --ifuel 1 --z3rlimit 15"
+open Core
+open FStar.Mul
+
+let _ =
+  (* This module has implicit dependencies, here we make them explicit. *)
+  (* The implicit dependencies arise from typeclasses instances. *)
+  let open Sandwich.Error in
+  let open Sandwich.Error.Code in
+  ()
+
+/// Returns the cipher name in the OpenSSL format.
+val cipher_name
+      (#impl_488124255_: Type0)
+      {| i1: Core.Convert.t_AsRef impl_488124255_ string |}
+      (name: impl_488124255_)
+    : Prims.Pure (Core.Option.t_Option string) Prims.l_True (fun _ -> Prims.l_True)
+
+/// Returns the library where a given error occurred.
+/// This function reproduces the `ERR_GET_LIB` method from OpenSSL, which
+/// is a static function in header (thus not understandable by bindgen).
+val err_get_lib (err: u64) : Prims.Pure i32 Prims.l_True (fun _ -> Prims.l_True)
+
+/// Returns the reason of why a given error occurred.
+/// This function reproduces the `ERR_GET_REASON` method from OpenSSL, which
+/// is a static function in header (thus not understandable by bindgen).
+val err_get_reason (err: u64) : Prims.Pure i32 Prims.l_True (fun _ -> Prims.l_True)
+
+let errstr__DEFAULT_BUFFER_LEN: usize = sz 256
+
+/// Tells if a BIO has reached EOF.
+val is_BIO_eof (bio: Core.Ptr.Non_null.t_NonNull Openssl3.t_bio_st)
+    : Prims.Pure bool Prims.l_True (fun _ -> Prims.l_True)
+
+/// Returns the last error.
+val peek_last_error: Prims.unit -> Prims.Pure u64 Prims.l_True (fun _ -> Prims.l_True)
+
+/// Returns a string containing the error strings for all errors that
+/// OpenSSL 3 has recorded.
+/// This function clears the error queue.
+val errstr: Prims.unit -> Prims.Pure Alloc.String.t_String Prims.l_True (fun _ -> Prims.l_True)
+
+/// Creates a `BIO` object from a immutable buffer.
+val v_BIO_from_buffer
+      (#impl_424714745_: Type0)
+      {| i1: Core.Convert.t_AsRef impl_424714745_ (t_Slice u8) |}
+      (buffer: impl_424714745_)
+    : Prims.Pure
+      (Core.Result.t_Result (Sandwich.Support.Pimpl.t_Pimpl Openssl3.t_bio_st)
+          Sandwich.Error.t_Error) Prims.l_True (fun _ -> Prims.l_True)
+
+/// Creates a new `BIO` object with a specific method.
+val new_BIO (bio_meth: Core.Ptr.Non_null.t_NonNull Openssl3.t_bio_method_st)
+    : Prims.Pure
+      (Core.Result.t_Result (Sandwich.Support.Pimpl.t_Pimpl Openssl3.t_bio_st)
+          Sandwich.Error.t_Error) Prims.l_True (fun _ -> Prims.l_True)
+
+/// Reads a private key (`EVP_PKEY` object) from a `BIO` object.
+val v_EVP_PKEY_from_BIO
+      (lib_ctx: Sandwich.Implementation.Openssl3.t_LibCtx)
+      (bio: Core.Ptr.Non_null.t_NonNull Openssl3.t_bio_st)
+      (format: Sandwich_api_proto.Encoding_format.t_ASN1EncodingFormat)
+    : Prims.Pure
+      (Core.Result.t_Result (Sandwich.Support.Pimpl.t_Pimpl Openssl3.t_evp_pkey_st)
+          Sandwich.Error.t_Error) Prims.l_True (fun _ -> Prims.l_True)
+
+/// Reads a certificate (`X509` object) from a `BIO` object.
+val v_X509_from_BIO
+      (lib_ctx: Sandwich.Implementation.Openssl3.t_LibCtx)
+      (bio: Core.Ptr.Non_null.t_NonNull Openssl3.t_bio_st)
+      (format: Sandwich_api_proto.Encoding_format.t_ASN1EncodingFormat)
+    : Prims.Pure
+      (Core.Result.t_Result (Sandwich.Support.Pimpl.t_Pimpl Openssl3.t_x509_st)
+          Sandwich.Error.t_Error) Prims.l_True (fun _ -> Prims.l_True)
