proofs/fstar/extraction/Sandwich.Support.Pimpl.fsti
@@ -1,0 +1,51 @@
+module Sandwich.Support.Pimpl
+#set-options "--fuel 0 --ifuel 1 --z3rlimit 15"
+open Core
+open FStar.Mul
+
+(* item error backend: (reject_RawOrMutPointer) ExplicitRejection { reason: "a node of kind [Raw_pointer] have been found in the AST" }
+Last available AST for this item:
+
+/// Wrapper around an raw pointer.
+#[allow(dead_code)]
+#[allow(unused_imports)]
+#[allow(dead_code)]
+#[deny(bare_trait_objects)]
+#[feature(register_tool)]
+#[register_tool(_hax)]
+struct t_Pimpl<'a: 'unk, T>
+where
+    _: core::marker::t_Sized<T>,
+{
+    /// The type to own.
+    f_p: core::ptr::non_null::t_NonNull<T>,
+    /// The deleter to call on the type.
+    f_del: core::option::t_Option<arrow!(raw_pointer!() -> tuple0)>,
+    /// A `PhantomData` to explicit the lifetime of the pointer.
+    f_phantom: core::marker::t_PhantomData<&T>,
+}
+
+
+Last AST:
+/** print_rust: pitem: not implemented  (item: { Concrete_ident.T.def_id =
+  { Concrete_ident.Imported.krate = "sandwich";
+    path =
+    [{ Concrete_ident.Imported.data =
+       (Concrete_ident.Imported.TypeNs "support"); disambiguator = 0 };
+      { Concrete_ident.Imported.data =
+        (Concrete_ident.Imported.TypeNs "pimpl"); disambiguator = 0 };
+      { Concrete_ident.Imported.data =
+        (Concrete_ident.Imported.TypeNs "Pimpl"); disambiguator = 0 }
+      ]
+    };
+  kind = Concrete_ident.Kind.Value }) */
+const _: () = ();
+ *)
+
+/// Returns a copy of the [`NonNull`] pointer.
+val impl_2__as_nonnull (#v_T: Type0) (self: t_Pimpl v_T)
+    : Prims.Pure (Core.Ptr.Non_null.t_NonNull v_T) Prims.l_True (fun _ -> Prims.l_True)
+
+/// Returns the raw pointer by consuming the object.
+val impl_2__into_raw (#v_T: Type0) (self: t_Pimpl v_T)
+    : Prims.Pure Rust_primitives.Hax.t_failure Prims.l_True (fun _ -> Prims.l_True)
