proofs/fstar/extraction/Sandwich.fsti
@@ -1,0 +1,16 @@
+module Sandwich
+#set-options "--fuel 0 --ifuel 1 --z3rlimit 15"
+open Core
+open FStar.Mul
+
+/// Top-level context.
+/// This context is used to create tunnel contexts.
+type t_Context = { f_ossl3_lib_ctx:Sandwich.Implementation.Openssl3.t_LibCtx }
+
+[@@ FStar.Tactics.Typeclasses.tcinstance]
+let impl_2: Core.Borrow.t_Borrow t_Context Sandwich.Implementation.Openssl3.t_LibCtx =
+  {
+    f_borrow_pre = (fun (self: t_Context) -> true);
+    f_borrow_post = (fun (self: t_Context) (out: Sandwich.Implementation.Openssl3.t_LibCtx) -> true);
+    f_borrow = fun (self: t_Context) -> self.f_ossl3_lib_ctx
+  }
